\begin{tabular}{l l l}
$\mathcal{I} \llbracket e \rrbracket$ &
$\Rightarrow$ &
$e$ \\ & & if $e$ is a value\\

$\mathcal{I} \llbracket C(e_1, \ldots, e_n) \rrbracket$ &
$\Rightarrow$ &
$C(\mathcal{I} \llbracket e_1 \rrbracket, \ldots, \mathcal{I} \llbracket e_n \rrbracket)$ \\

$\mathcal{I} \llbracket con \langle f(e_1, \ldots, e_n) \rangle \rrbracket$ &
$\Rightarrow$ &
$\mathcal{I} \llbracket con \langle e \{v_1 := e_1, \ldots, v_n := e_n\} \rangle \rrbracket$ \\
& & when $f(x_1, \ldots, x_n) \stackrel{\textrm{\tiny p}}{=} e$\\

$\mathcal{I} \llbracket con \langle g(C(e_1, \ldots, e_m), e_{m+1},\ldots, e_n)\rangle \rrbracket$ &
$\Rightarrow$ &
$\mathcal{I} \llbracket con \langle e \{v_1 := e_1, \ldots, v_n := e_n\} \rangle \rrbracket$ \\
& & when $g(C(v_1, \ldots, v_m), v_{m+1},\ldots, v_n) \stackrel{\textrm{\tiny p}}{=} e$ 
\end{tabular}